---
layout: article
title: Lecture 19:Duality--Dual Problem
tags: Linear_Programming
aside:
  toc: true
sidebar:
  nav: Linear_Programming
---

In the end of the series of LP blogs, we will introduce a very important structure in LP problem, that is the dual problem. Dual problem can give us another view of a LP problem. There are a lot of applications of Duality in algorithm, like Max flow and Min Cut problem. Additionally, you can find more application of primal-dual techniques in my another [blog series](https://wu-haonan.github.io/2023/09/27/ADA_Lec_11.html).   



In this blog, we will first introduce what is dual problem, how to convert the primal problem to its dual problem.

<!--more-->

# Dual problem

Given matrix $A$ represented as:

$$
A = 
\begin{bmatrix}
\bar{a}^\top_1 \\
\bar{a}^\top_2 \\
\vdots \\
\bar{a}^\top_m \\
\end{bmatrix}
= [\bar{A}_1, \bar{A}_2, \ldots, \bar{A}_n]
$$

where $\bar{b} \in \mathbb{R}^m$ and $\bar{c} \in \mathbb{R}^n$.

**(a) PRIMAL PROBLEM**
$$
\begin{aligned}
&\text{Minimize} \quad & \bar{c}^\top \bar{x} && \\
&\text{subject to} & \bar{a}_i^\top \bar{x} \geq b_i; && i \in M_1, \\
&& \bar{a}_i^\top \bar{x} \leq b_i; && i \in M_2, \\
&& \bar{a}_i^\top \bar{x} = b_i; && i \in M_3, \\
&& \bar{x}_j \geq 0; && j \in N_1, \\
&& \bar{x}_j \leq 0; && j \in N_2, \\
&& \bar{x}_j \in \mathbb{R}; && j \in N_3.
\end{aligned}
$$

**(b) DUAL PROBLEM**
$$
\begin{aligned}
&\text{Maximize} \quad & \bar{p}^\top \bar{b} &&\\
&\text{subject to} & \bar{p}_i \geq 0; && i \in M_1, \\
&& \bar{p}_i \leq 0; && i \in M_2, \\
&& \bar{p}_i \in \mathbb{R}; && i \in M_3, \\
&& \bar{p}^\top \bar{A}_j \leq c_j; && j \in N_1, \\
&& \bar{p}^\top \bar{A}_j \geq c_j; && j \in N_2, \\
&& \bar{p}^\top \bar{A}_j = c_j; && j \in N_3.
\end{aligned}
$$

For each constraint in the primal (other than sign constraints), we introduce a variable in the dual problem. For each variable in the primal, we introduce a constraint in the dual. 

* Depending on whether the primal constraint is an equality or inequality constraint, the corresponding dual variable is either free or sign-constrained, respectively.

* Depending on whether a variable in the primal problem is free or sign-constrained, we have either an equality or an inequality constraint, respectively, in the dual problem.

**Relations between primal and dual variables and constraints**

| Primal | $\min \quad \bar{c}^\top \bar{x}$ | $\max \quad \bar{p}^\top \bar{b}$ | Dual |
|:------:|:-:|:-:|:----:|
| Constraints | $ \begin{aligned} \bar{a}_i^\top \bar{x} & \geq b_i \\ \bar{a}_i^\top \bar{x} & \leq b_i \\ \bar{a}_i^\top \bar{x} & = b_i \end{aligned} $ |$\begin{aligned} p_i & \geq 0 \\ p_i & \leq 0 \\ p_i &\text{ free}   \end{aligned}$|Variables|
| Variables | $\begin{aligned} x_j & \geq 0 \\ x_j & \leq 0 \\ x_j &\text{ free}   \end{aligned}$ |$\begin{aligned} \bar{p}^\top \bar{A}_j & \leq c_j \\ \bar{p}^\top \bar{A}_j & \geq c_j \\ \bar{p}^\top \bar{A}_j & = c_j \end{aligned} $ |Constraints |

Every maximization problem can always be converted into an equivalent minimization problem and conversely. However, to avoid confusion, we will adhere to the convention that the primal is a minimization problem and its dual is a maximization problem.

# Involution and Equivalency

## Dual of Dual is Primal

**Theorem:** The dual of the dual is the primal. If we transform the dual into an equivalent minimization problem and then find its dual, we obtain a problem equivalent to the original (primal) problem.

**Proof:**

Let's give a **primal problem**:

$$
\begin{aligned}
&\text{Minimize} \quad & \bar{c}^\top \bar{x} && \\
&\text{subject to} & \bar{a}_i^\top \bar{x} \geq b_i; && i \in M_1, \\
&& \bar{a}_i^\top \bar{x} \leq b_i; && i \in M_2, \\
&& \bar{a}_i^\top \bar{x} = b_i; && i \in M_3, \\
&& \bar{x}_j \geq 0; && j \in N_1, \\
&& \bar{x}_j \leq 0; && j \in N_2, \\
&& \bar{x}_j \in \mathbb{R}; && j \in N_3.
\end{aligned}
$$

Then we can give the **dual problem** by definition:

$$
\begin{aligned}
&\text{Maximize} \quad & \bar{p}^\top \bar{b} &&\\
&\text{subject to} & \bar{p}_i \geq 0; && i \in M_1, \\
&& \bar{p}_i \leq 0; && i \in M_2, \\
&& \bar{p}_i \in \mathbb{R}; && i \in M_3, \\
&& \bar{p}^\top \bar{A}_j \leq c_j; && j \in N_1, \\
&& \bar{p}^\top \bar{A}_j \geq c_j; && j \in N_2, \\
&& \bar{p}^\top \bar{A}_j = c_j; && j \in N_3.
\end{aligned}
$$

**Equivalent reformulation** of the dual problem involves renaming the decision variables $\bar{q} = \bar{p}$ and transforming the objective function by $c \rightarrow -c$ transforms min into max:
$$
\begin{aligned}
&\text{Maximize} \quad & -\bar{b}^\top \bar{q} &&\\
&\text{subject to} & \bar{q}_i \geq 0; && i \in M_1, \\
&& \bar{q}_i \leq 0; && i \in M_2, \\
&& \bar{q}_i \in \mathbb{R}; && i \in M_3, \\
&& (-\bar{A}_j)^\top \bar{q}  \geq -c_j; && j \in N_1, \\
&& (-\bar{A}_j)^\top \bar{q}  \leq- c_j; && j \in N_2, \\
&& (-\bar{A}_j)^\top \bar{q}  = -c_j; && j \in N_3.
\end{aligned}
$$

The **dual of this equivalent reformulation** yields following problem:

$$
\begin{aligned}
&\text{Maximize} \quad & \bar{x}^\top (-\bar{c}) && \\
&\text{subject to} &  \bar{x}^\top (-\bar{a}_i) \leq -b_i; && i \in M_1, \\
&& \bar{x}^\top (-\bar{a}_i) \geq -b_i; && i \in M_2, \\
&& \bar{x}^\top (-\bar{a}_i) = -b_i; && i \in M_3, \\
&& \bar{x}_j \geq 0; && j \in N_1, \\
&& \bar{x}_j \leq 0; && j \in N_2, \\
&& \bar{x}_j \in \mathbb{R}; && j \in N_3.
\end{aligned}
$$

The above problem is exactly the primal problem by **equivalent reformulation**. Hence, we have the dual of the dual is the primal. $\square$

## Dual of equivalent problems are equivalent

**Theorem:** The duals of equivalent problems are equivalent. Suppose that we have transformed a LP problem $\Pi_1$ to another (equivalent) LP problem $\Pi_2$ by a sequence of transformations of the following types:

(a) Replace a variable $x$ unrestricted in sign with the difference $x^+ - x^-$ of two nonnegative variables.

(b) Replace an inequality constraint (e.g. $\bar{a}^\top \bar{x} \leq b$) by an equality constraint involving a nonnegative slack variable (e.g. $\bar{a}^\top \bar{x} + s = b$ with $s \geq 0$).

(c) If some row of the constraint matrix $A$ in a feasible standard form problem is a linear combination of the other rows of $A$, eliminate the corresponding equality constraint.

Then, the duals of $\Pi_1$ and $\Pi_2$ are equivalent, i.e. they are either both infeasible or they have the same optimal cost.

**Proof:** 

Consider the primal problem shown on the left and its dual shown on the right:

$$
\begin{equation}
\begin{aligned}
\text{minimize} \quad & \bar{c}^\top \bar{x} \\
\text{subject to} \quad & A\bar{x} \geq \bar{b} \\
& \bar{x} \text{ free}
\end{aligned}
\quad \quad
\begin{aligned}
\text{maximize} \quad & \bar{p}^\top \bar{b} \\
\text{subject to}  \quad & \bar{p} \geq \bar{0} \\
 & \bar{p}^\top A = \bar{c}^\top
\end{aligned}
\end{equation}
$$

We transform the primal problem by introducing surplus variables and then obtain its dual:


$$
\begin{equation}
\begin{aligned}
\text{minimize} \quad & \bar{c}^\top \bar{x} + \bar{0}^\top \bar{s} \\
\text{subject to} \quad & A\bar{x} - I \bar{s} = \bar{b} \\
& \bar{s} \geq \bar{0} \\
& \bar{x} \text{ free} 
\end{aligned}
\quad \quad 
\begin{aligned}
\text{maximize} \quad & \bar{p}^\top \bar{b} \\
\text{subject to} \quad & \bar{p} \text{ free} \\
& \bar{p}^\top (-I) \leq \bar{0}^\top \\
& \bar{p}^\top A = \bar{c}^\top
\end{aligned}
\end{equation}
$$

We observe that the constraint $\bar{p} \geq \bar{0}$ is equivalent to the constraint $\bar{p} (- I) \leq \bar{0}$. **Note** the above dual problem of adding surplus variables is equivalent to the dual problem of primal problem, which implies **operation (a) will not change equivalency**. 



Alternatively, if we take the original primal problem and replace $\bar{x}$ by sign-constrained variables, we obtain the following pair of problems:

$$
\begin{equation}
\begin{aligned}
\text{minimize} \quad & \bar{c}^\top \bar{x}^+ - \bar{c}^\top \bar{x}^- \\
\text{subject to} \quad & A\bar{x}^+ - A\bar{x}^- \geq \bar{b} \\
& \bar{x}^+ \geq \bar{0} \\
& \bar{x}^- \geq \bar{0}
\end{aligned}
\quad \quad
\begin{aligned}
\text{maximize} \quad & \bar{p}^\top \bar{b} \\
\text{subject to} \quad & \bar{p} \geq \bar{0} \\
& \bar{p}^\top A \leq \bar{c}^\top \\
& \bar{p}^\top (-A) \leq -\bar{c}^\top \\
\end{aligned}
\end{equation}
$$

Notice that the constraint $\bar{p}^\top A = \bar{c}^\top$ is equivalent to the two constraints $\bar{p}^\top A \leq \bar{c}^\top$ and $\bar{p}^\top (-A) \leq -\bar{c}^\top$. Thus, we have equivalent forms of the primal, which implies **operation (b) will not change equivalency**. 



Now, we can consider a standard form problem, assumed feasible, and its dual:

$$
\begin{equation}
\begin{aligned}
\text{minimize} \quad & \bar{c}^\top \bar{x} \\
\text{subject to} \quad & A\bar{x} = \bar{b} \\
& \bar{x} \geq \bar{0}
\end{aligned}
\quad \quad
\begin{aligned}
\text{maximize} \quad & \bar{p}^\top \bar{b} \\
\text{subject to} \quad &  \bar{p} \text{ free}\\
& \bar{p}^\top A \leq \bar{c}^\top
\end{aligned}
\end{equation}
$$

Let $\bar{a}\_1, ..., \bar{a}\_m$ be the rows of $A$ and suppose that $\bar{a}_m = \sum\_{i=1}^{m-1} \lambda_i \bar{a}_i$ for some scalars $\lambda\_1, ..., \lambda\_{m-1}$, that means the last equality constraint is redundant and can be eliminated. 

By considering an arbitrary feasible solution $\bar{x}$, we obtain 

$$
b_m = \bar{a}_m^\top \bar{x} = (\sum_{i=1}^{m-1} \lambda_i \bar{a}_i^\top)\bar{x} =  \sum_{i=1}^{m-1} \lambda_i b_i
$$

Note that the **dual constraints** are of the form $ \sum_{i=1}^m p_i \bar{a}_i^\top \leq \bar{c}^\top $ and can be rewritten as 

$$
\sum_{i=1}^{m-1} (p_i + p_m \lambda_i) \bar{a}_i \leq \bar{c}^\top
$$

Furthermore, using $b_m = \sum_{i=1}^{m-1} \lambda_i b_i$, the **dual cost** $\sum p_i b_i$ is equal to $\sum_{i=1}^{m-1} (p_i + p_m \lambda_i) b_i$.

If we now let $\bar{q}_i = \bar{p}_i + \bar{p}_m\lambda_i$, we see that the dual problem is equivalent to:

$$
\begin{aligned}
\text{maximize} \quad & \sum_{i=1}^{m-1} \bar{q}_i b_i \\
\text{subject to} \quad & \sum_{i=1}^{m-1} \bar{q}_i \bar{a}_i^\top \leq \bar{c}^\top.
\end{aligned}
$$

We observe that this is the exact same dual that we would have obtained if we had eliminated the last (and redundant) constraint in the primal problem, before forming the dual. $\square$
